Term/WithArity/ABinary.v
@@ -1,0 +1,187 @@
+(**
+CoLoR, a Coq library on rewriting and termination.
+See the COPYRIGHTS and LICENSE files.
+
+- Sidi Ould-Biha, 2010-05-04
+
+properties of signatures with a symbol of arity 2
+*)
+
+Set Implicit Arguments.
+
+Require Import ATrs VecUtil ListUtil LogicUtil NatUtil RelUtil.
+
+Record BinSignature : Type := Make {
+  Sig :> Signature;
+  Cons : Sig;
+  _ : arity Cons = 2
+}.
+
+Section BinSignatureTheory.
+
+  Variable Sig : BinSignature.
+
+  Notation term := (term Sig). Notation terms := (vector term).
+  Notation rule := (rule Sig). Notation rules := (list rule).
+
+  Lemma cons_arity : 2 = arity (Cons Sig).
+
+  Proof. case Sig. auto. Qed.
+
+  (* Building a new term with Cons as root symbol *)
+  Fixpoint cons_term (t : term) n (v : terms n) : term :=
+    match v with 
+      | Vnil => t
+      | Vcons t' _ v' => Fun (Cons Sig)
+        (Vcast (Vcons t (Vcons (cons_term t' v') Vnil)) cons_arity)
+    end.
+
+  Lemma cons_term_cons : forall t t' n (v : terms n),
+    cons_term t (Vcons t' v)
+    = Fun (Cons Sig) (Vcast (Vcons t (Vcons (cons_term t' v) Vnil)) cons_arity).
+
+  Proof. intros. auto. Qed.
+
+  (* Projection TRS associated to Cons *)
+  Definition proj_cons : rules :=
+    let Vxy := Vcast (Vcons (Var 0) (Vcons (Var 1) Vnil)) cons_arity in
+      mkRule (Fun (Cons Sig) Vxy) (Var 0)
+      :: mkRule (Fun (Cons Sig) Vxy) (Var 1) :: nil.
+
+  Lemma proj_cons_l : forall n (v : terms n) t a,
+    red proj_cons (cons_term t (Vcons a v)) t.
+
+  Proof.
+    pose (Vxy := (Vcast (Vcons (Var 0) (Vcons (@Var Sig 1) Vnil)) cons_arity)).
+    intros. exists (Fun (Cons Sig) Vxy). exists (Var 0). exists Hole.
+    pose (s := fun i => match i with | 0 => t | S j => match j with
+      | 0 => (cons_term a v) | S k => t end end).
+    exists s. split. unfold proj_cons. rewrite In_cons. left. refl.
+    split. Focus 2. simpl; auto. rewrite cons_term_cons. unfold Vxy.
+    apply args_eq. apply Veq_nth. intros i Hi. rewrite Vnth_map, !Vnth_cast.
+    destruct i. simpl; refl. rewrite !Vnth_cons. destruct i. simpl; refl.
+    cut (S (S i) < 2). intro; absurd_arith. rewrite cons_arity; auto.
+  Qed.
+
+  Lemma proj_cons_r : forall n (v : terms n) t a,
+    red proj_cons (cons_term t (Vcons a v)) (cons_term a v).
+
+  Proof.
+    pose (Vxy := (Vcast (Vcons (Var 0) (Vcons (@Var Sig 1) Vnil)) cons_arity)).
+    intros. exists (Fun (Cons Sig) Vxy). exists (Var 1). exists Hole.
+    pose (s := fun i => match i with | 0 => t | S j => match j with
+      | 0 => (cons_term a v) | S k => t end end). exists s. split.
+    unfold proj_cons. rewrite In_cons. right. rewrite In_cons. left; refl.
+    split. Focus 2. simpl; auto. rewrite cons_term_cons. unfold Vxy.
+    apply args_eq. apply Veq_nth. intros i Hi. rewrite Vnth_map, !Vnth_cast.
+    destruct i. simpl; refl. rewrite !Vnth_cons. destruct i. simpl; refl.
+    cut (S (S i) < 2). intro; absurd_arith. rewrite cons_arity; auto.
+  Qed.
+
+  Lemma proj_cons_rtc_l : forall t n (v : terms n),
+    red proj_cons # (cons_term t v) t.
+
+  Proof.
+    intros. case v. simpl. apply rt_refl.
+    intros t' n' v'. apply rt_step. apply proj_cons_l.
+  Qed.
+
+  Lemma proj_cons_tc_r : forall n (v : terms n) t x,
+    Vin x v -> red proj_cons ! (cons_term t v) x.
+
+  Proof.
+    intro n. induction v; intros. simpl in H. tauto.
+    apply tc_merge. exists (cons_term a v). split. apply proj_cons_r.
+    destruct H. rewrite H. apply proj_cons_rtc_l.
+    apply tc_incl_rtc. apply IHv; auto.
+  Qed.
+
+  Lemma proj_cons_fun_aux1 : forall f n m (Emn : n + S m = arity f) v1 v2 x y,
+    red proj_cons # x y ->
+      red proj_cons # (Fun f (Vcast (Vapp v1 (Vcons x v2)) Emn))
+                      (Fun f (Vcast (Vapp v1 (Vcons y v2)) Emn)).
+
+  Proof.
+    intros f m n. induction 1. Focus 2. apply rt_refl. apply rt_step.
+    destruct H as [l H]; destruct H as [r H]; destruct H as [c H].
+    destruct H as [s H]. exists l. exists r.
+    exists (Cont _ Emn v1 c v2). exists s. split. destruct H; auto. simpl.
+    destruct H as [_ H]. destruct H as [H3 H4]. rewrite <- H3, <- H4. auto.
+    apply rt_trans with (y := Fun f (Vcast (Vapp v1 (Vcons y v2)) Emn)); auto.
+  Qed.
+
+  Lemma proj_cons_fun_aux2 : forall f n m (Emn : n + m = arity f) v v1 v2,
+    (forall i (Hi : i < n), red proj_cons # (Vnth v1 Hi) (Vnth v2 Hi))
+    -> red proj_cons # (Fun f (Vcast (Vapp v1 v) Emn))
+                       (Fun f (Vcast (Vapp v2 v) Emn)).
+
+  Proof.
+    intro f. induction n; intros m Emn v v1 v2 Hin.
+    rewrite (VO_eq v1), (VO_eq v2). simpl. apply rt_refl.
+    assert (H0 : n < S n + m). omega. assert (H1 : m = S n + m - S n). omega.
+    rewrite (Veq_app_cons (Vapp v1 v) H0), (Veq_app_cons (Vapp v2 v) H0).
+    assert (Ve1 : forall x,
+      Vsub (Vapp x v) (Veq_app_cons_aux2 H0) = (Vcast v H1)).
+    intro x; pattern v at 2. rewrite <- (Vsub_app_r x v (le_refl (S n + m))).
+    rewrite Vcast_sub. apply Vsub_pi.
+    assert (Ve2 : forall x, Vsub (Vapp x v) (Veq_app_cons_aux1 H0) =
+      (Vsub x (Veq_app_aux1 (le_n_Sn n)))). intro x.
+    apply Veq_nth; intros. rewrite !Vnth_sub, Vnth_app.
+    case (le_gt_dec (S n) (0 + i)); intro. absurd_arith. apply Vnth_eq; auto.
+    rewrite (Ve1 v1), (Ve1 v2), (Ve2 v1), (Ve2 v2), !Vnth_app.
+    rewrite !Vcast_cast. case (le_gt_dec (S n) n); intro H2. absurd_arith.
+    set (v' := Vcast v H1); set (x := Vnth v1 H2); set (y := Vnth v2 H2).
+    set (v1' := Vsub v1 (Veq_app_aux1 (le_n_Sn n))).
+    set (v2' := Vsub v2 (Veq_app_aux1 (le_n_Sn n))).
+    set (H3 := trans_eq (Veq_app_cons_aux3 H0) Emn).
+    apply rt_trans with (y := Fun f (Vcast (Vapp v2' (Vcons x v')) H3)).
+    apply IHn. intros. unfold v1', v2'. rewrite !Vnth_sub. apply Hin.
+    apply proj_cons_fun_aux1. apply Hin.
+  Qed.
+
+  Lemma proj_cons_fun : forall f v1 v2,
+    (forall i (Hi : i < arity f), red proj_cons # (Vnth v1 Hi) (Vnth v2 Hi))
+    -> red proj_cons # (Fun f v1) (Fun f v2).
+
+  Proof.
+    intros. generalize (proj_cons_fun_aux2 f (plus_0_r (arity f)) Vnil v1 v2 H).
+    rewrite !Vapp_nil, !Vcast_cast, !Vcast_refl; auto.
+  Qed.
+
+End BinSignatureTheory.
+
+(***********************************************************************)
+(** extend a signature with a binary symbol *)
+
+Section MakeExtSig.
+
+  Variable Sig : Signature.
+
+  Inductive ext_symb : Type := Symb : Sig -> ext_symb | Pair : ext_symb.
+
+  Definition ext_arity f :=
+    match f with
+      | Symb f => arity f
+      | Pair => 2
+    end.
+
+  Definition beq_ext_symb f g :=
+    match f, g with
+      | Symb f', Symb g' => beq_symb f' g'
+      | Pair, Pair => true
+      | _, _ => false
+    end.
+
+  Lemma beq_ext_symb_ok : forall f g, beq_ext_symb f g = true <-> f = g.
+
+  Proof.
+    destruct f; destruct g; simpl.
+    rewrite beq_symb_ok. intuition. subst s0. refl. inversion H. refl.
+    intuition. discr. intuition. discr. tauto.
+  Qed.
+
+  Definition ext_sig := mkSignature ext_arity beq_ext_symb_ok.
+
+  Definition ext := Make ext_sig Pair (refl_equal 2).
+
+End MakeExtSig.
